Test/mytest/seq.dfy
@@ -1,0 +1,10 @@
+function sorted(s: seq<int>): bool
+{
+forall i,j :: 00 <= i < j < |s| ==> s[i] <= s[j]
+}
+
+
+method m()
+{
+  assert sorted([1,2]);
+}
